clean

experiments/mst_handleaway/MST.Tot.fst
@@ -1,17 +1,14 @@
 module MST.Tot
 
+
+open FStar.Tactics
 open MST
 open FStar.Preorder
 open FStar.Monotonic.Heap
 
 module W = FStar.Monotonic.Witnessed
-  
-let st_pre           = st_pre_h heap
-let st_post' (a:Type) (pre:Type) = st_post_h' heap a pre
-let st_post  (a:Type) = st_post_h heap a
-let st_wp (a:Type)   = st_wp_h heap a
 
-(* Total state effect --- this means that the heap is first-order *)
+(* Total state effect --- the heap is first-order *)
 
 let heap_rel (h1:heap) (h2:heap) =
   forall (a:Type0) (rel:preorder a) (r:mref a rel). h1 `contains` r ==>
@@ -21,36 +18,58 @@ let heap_state : tstate = { t = heap; rel = heap_rel }
 
 let stable (pred:heap_state.t -> Type0) = stable pred heap_state.rel
 
-let _mst a (wp:st_wp a) = mst heap_state a wp
-let _mst_bind a b wp_v wp_f v f = mst_bind #heap_state #a #b #wp_v #wp_f v f
-let _mst_return a x = mst_return #heap_state #a x
+let st_pre   = st_pre_h   heap_state.t
+let st_post' = st_post_h' heap_state.t
+let st_post  = st_post_h  heap_state.t
+let st_wp    = st_mwp_h   heap_state.t
 
-let _mst_subcomp a (wp1:st_wp heap_state.t a) (wp2:st_wp heap_state.t a) v:
-  Pure (_mst a wp2) (requires (wp1 ⊑ wp2)) (ensures (fun _ -> True)) = 
-  mst_subcomp #heap_state #a #wp1 #wp2 v
+val mheap : (a:Type u#a) -> st_wp a -> Type u#(max 1 a)
+let mheap = mst heap_state
 
-let _mst_if_then_else (a : Type u#a)
-  (#wp1 : st_wp heap_state.t a)
-  (#wp2 : st_wp heap_state.t a)
-  (f : _mst a wp1) (g : _mst a wp2) (b : bool) : Type =
-  _mst a (st_if_then_else heap_state.t a b wp1 wp2)
+val mheap_bind :
+  (a : Type u#a) ->
+  (b : Type u#b) ->
+  (wp_v : st_wp a) ->
+  wp_f: (a -> st_wp b) ->
+  (v : mheap a wp_v) ->
+  (f : (x:a -> mheap b (wp_f x))) ->
+  Tot (mheap b (st_bind_wp heap_state.t a b wp_v wp_f))
+let mheap_bind a b wp_v wp_f v f = mst_bind #heap_state #a #b #wp_v #wp_f v f
+
+val mheap_return : (a:Type) -> (x:a) -> mheap a (st_return heap_state.t a x)
+let mheap_return a = mst_return #heap_state #a
+
+
+val mheap_subcomp :
+  (a : Type u#a) ->
+  (wp1 : st_wp a) ->
+  (wp2 : st_wp a) ->
+  (v : mheap a wp1) ->
+  Pure (mheap a wp2) (requires (wp1 ⊑ wp2)) (ensures (fun _ -> True))
+let mheap_subcomp a wp1 wp2 = mst_subcomp #heap_state #a #wp1 #wp2
+
+let mheap_if_then_else (a : Type u#a)
+  (#wp1 : st_wp a)
+  (#wp2 : st_wp a)
+  (f : mheap a wp1) (g : mheap a wp2) (b : bool) : Type =
+  mheap a (st_if_then_else heap_state.t a b wp1 wp2)
 
 total
 reifiable
 reflectable
 effect {
-  STATEwp (a:Type) (wp : st_wp heap_state.t a)
+  STATEwp (a:Type) (wp : st_wp a)
   with {
-       repr       = _mst
-     ; return     = _mst_return
-     ; bind       = _mst_bind
-     ; subcomp    = _mst_subcomp
-     ; if_then_else = _mst_if_then_else
+       repr       = mheap
+     ; return     = mheap_return
+     ; bind       = mheap_bind
+     ; subcomp    = mheap_subcomp
+     ; if_then_else = mheap_if_then_else
      }
 }
 
 unfold
-let wp_lift_pure_st (w : pure_wp 'a) : st_wp heap_state.t 'a =
+let wp_lift_pure_st (w : pure_wp 'a) : st_wp 'a =
   FStar.Monotonic.Pure.elim_pure_wp_monotonicity_forall ();
   fun p h -> w (fun r -> p r h)
 
@@ -58,20 +77,20 @@ val lift_pure_mst :
   a: Type u#a ->
   w: pure_wp a ->
   f: (eqtype_as_type unit -> PURE a w) ->
-  Tot (_mst a (wp_lift_pure_st w))
+  Tot (mheap a (wp_lift_pure_st w))
 let lift_pure_mst a w f =
   FStar.Monotonic.Pure.elim_pure_wp_monotonicity_forall ();
   let lhs = partial_return heap_state (as_requires w) in
-  let rhs = (fun (pre:(squash (as_requires w))) -> _mst_return a (f pre)) in
-  let m = _mst_bind _ _ _ _ lhs rhs in
-  _mst_subcomp _ _ _ m
+  let rhs = (fun (pre:(squash (as_requires w))) -> mheap_return a (f pre)) in
+  let m = mheap_bind _ _ _ _ lhs rhs in
+  mheap_subcomp _ _ _ m
 
 sub_effect PURE ~> STATEwp = lift_pure_mst
 
-let get () : STATEwp heap get_wp = 
+let get () : STATEwp heap (get_wp #heap_state) = 
   STATEwp?.reflect (mst_get ())
 
-let put (h1:heap) : STATEwp unit (put_wp h1) = 
+let put (h1:heap) : STATEwp unit (put_wp #heap_state h1) = 
   STATEwp?.reflect (mst_put h1)
 
 type heap_predicate = heap -> Type0
@@ -91,13 +110,13 @@ effect ST (a:Type) (pre:st_pre) (post: (h:heap -> Tot (st_post' a (pre h)))) =
 effect St (a:Type) = ST a (fun h -> True) (fun h0 r h1 -> True)
 
 
-let contains_pred (#a:Type) (#rel:FStar.Preorder.preorder a) (r:mref a rel) = fun h -> h `contains` r
+let contains_pred (#a:Type) (#rel:preorder a) (r:mref a rel) = fun h -> h `contains` r
 
-type mref (a:Type0) (rel:FStar.Preorder.preorder a) =
+type mref (a:Type0) (rel:preorder a) =
   r:Heap.mref a rel{is_mm r = false /\ witnessed (contains_pred r)}
 
-let alloc (#a:Type) (#rel:FStar.Preorder.preorder a) (init:a)
-  :ST (mref a rel)
+let alloc (#a:Type) (#rel:preorder a) (init:a) :
+  ST (mref a rel)
       (fun h -> True)
       (fun h0 r h1 -> fresh r h0 h1 /\ modifies Set.empty h0 h1 /\ sel h1 r == init)
   = let h0 = get () in
@@ -106,13 +125,13 @@ let alloc (#a:Type) (#rel:FStar.Preorder.preorder a) (init:a)
     witness (contains_pred r);
     r
 
-let read (#a:Type) (#rel:FStar.Preorder.preorder a) (r:mref a rel) :STATEwp a (fun p h -> p (sel h r) h)
+let read (#a:Type) (#rel:preorder a) (r:mref a rel) :STATEwp a (fun p h -> p (sel h r) h)
   = let h0 = get () in
     recall (contains_pred r);
     Heap.lemma_sel_equals_sel_tot_for_contained_refs h0 r;
     sel_tot h0 r
 
-let write (#a:Type) (#rel:FStar.Preorder.preorder a) (r:mref a rel) (v:a)
+let write (#a:Type) (#rel:preorder a) (r:mref a rel) (v:a)
   : ST unit
     (fun h -> rel (sel h r) v)
     (fun h0 x h1 -> rel (sel h0 r) v /\ h0 `contains` r /\
@@ -126,11 +145,11 @@ let write (#a:Type) (#rel:FStar.Preorder.preorder a) (r:mref a rel) (v:a)
     Heap.lemma_upd_equals_upd_tot_for_contained_refs h0 r v;
     put h1
 
-let op_Bang (#a:Type) (#rel:FStar.Preorder.preorder a) (r:mref a rel)
+let op_Bang (#a:Type) (#rel:preorder a) (r:mref a rel)
   : STATEwp a (fun p h -> p (sel h r) h)
 = read #a #rel r
 
-let op_Colon_Equals (#a:Type) (#rel:FStar.Preorder.preorder a) (r:mref a rel) (v:a)
+let op_Colon_Equals (#a:Type) (#rel:preorder a) (r:mref a rel) (v:a)
   : ST unit
     (fun h -> rel (sel h r) v)
     (fun h0 x h1 -> rel (sel h0 r) v /\ h0 `contains` r /\
